examples/NSL/DY.NSL.Invariants.Proofs.fst
@@ -25,42 +25,94 @@ val send_msg1_invariant:
     trace_invariant tr_out
   ))
 
-let send_msg1_invariant alice bob alice_public_keys_sid tr =
-  let (n_a, tr_rand) = gen_rand_labeled (nonce_label alice bob) tr in
-  let msg1 = Msg1 {alice; n_a} in
-  serialize_wf_lemma message_t (is_knowable_by (nonce_label alice bob) tr_rand) msg1;
-  match pke_enc_for_is_publishable tr_rand alice bob alice_public_keys_sid key_tag msg1 with
-  | (None, tr_enc) -> (
-    assert(trace_invariant tr_rand);
-    assert(tr == tr_rand)
-  )
-  | (Some msg1_encrypted, tr_enc) -> (
+#push-options "--fuel 3 --ifuel 3 --z3rlimit 50"
+let send_msg1_invariant alice bob alice_public_keys_sid tr = (
+  let (msg_ts, tr_out) = send_msg1 alice alice_public_keys_sid bob tr in
+  match msg_ts with
+  | None -> admit()
+  | Some(_) -> (
+    let (n_a, tr_rand) = gen_rand_labeled (nonce_label alice bob) tr in
+    assert(is_secret (nonce_label alice bob) tr_rand n_a);
+    let init_event = Initiating{alice; bob; n_a} in
+    let (_, tr_event) = trigger_event alice init_event tr_rand in
+    assert(trace_invariant tr_event);
+    let msg1 = Msg1 {alice; n_a} in
+    let (Some(msg1_encrypted), tr_enc) = pke_enc_for alice bob alice_public_keys_sid key_tag msg1 tr_event in
     assert(trace_invariant tr_enc);
-    let (msg_ts, tr_msg) = send_msg msg1_encrypted tr_enc in
-    
+    assert(is_well_formed _ (bytes_invariant tr_event) msg1);
+    assert(is_well_formed _ (is_knowable_by (long_term_key_label bob) tr_event) msg1);
+    assert(is_well_formed _ (is_knowable_by (long_term_key_label alice) tr_event) msg1);
+    assert(has_pki_invariant);
+    assume(is_publishable tr msg1_encrypted);
+    let (msg1_ts, tr_send) = send_msg msg1_encrypted tr_enc in
+    assert(trace_invariant tr_send);
+    let msg1_state = SentMsg1 {bob; n_a} in
+    let (sid, tr_st) = start_new_session alice msg1_state tr_send in
+    assert(is_secret (nonce_label alice bob) tr_send n_a);
+    assert(trace_invariant tr_st);
+    assert(tr_st == tr_out);
+    ()
   )
+)
 
 val receive_msg1_and_send_msg2:
   alice:principal -> bob:principal -> bob_public_keys_sid:state_id -> bob_private_keys_sid:state_id -> msg1_ts:timestamp -> tr:trace ->
   Lemma
   (requires trace_invariant tr)
   (ensures (
-    let (_, tr_out) = receive_msg1_and_send_msg2 bob bob_private_keys_sid bob_public_keys_sid msg1_ts in
+    let (_, tr_out) = receive_msg1_and_send_msg2 bob bob_private_keys_sid bob_public_keys_sid msg1_ts tr in
     trace_invariant tr_out
   ))
 
-  let receive_msg1_and_send_msg2 alice bob bob_public_keys_sid bob_private_keys_sid msg1_ts tr = (admit())
+  let receive_msg1_and_send_msg2 alice bob bob_public_keys_sid bob_private_keys_sid msg1_ts tr = admit()
 
   val receive_msg2_and_send_msg3:
     alice:principal -> bob:principal -> alice_public_keys_sid:state_id -> alice_private_keys_sid:state_id -> msg2_ts:timestamp -> tr:trace ->
     Lemma
     (requires trace_invariant tr)
     (ensures (
-      let (_, tr_out) = receive_msg2_and_send_msg3 alice bob alice_private_keys_sid alice_public_keys_sid msg2_ts in
+      let (_, tr_out) = receive_msg2_and_send_msg3 alice alice_private_keys_sid alice_public_keys_sid msg2_ts tr in
       trace_invariant tr_out
     ))
 
-  let receive_msg2_and_send_msg3 alice bob alice_public_keys_sid alice_private_keys_sid msg2_ts tr = (admit())
+  let receive_msg2_and_send_msg3 alice bob alice_public_keys_sid alice_private_keys_sid msg2_ts tr = (
+    let (msg_ts, tr_out) = receive_msg2_and_send_msg3 alice alice_private_keys_sid alice_public_keys_sid msg2_ts tr in
+    assert(trace_invariant tr);
+    match msg_ts with
+    | None -> admit()
+    | Some(_) -> (
+      let (Some(msg2_encrypted), tr_rec) = recv_msg msg2_ts tr in
+      assert(trace_invariant tr_rec);
+      let (Some(msg2), tr_dec) = pke_dec_with_key_lookup #message_t alice alice_private_keys_sid key_tag msg2_encrypted tr_rec in
+      assert(trace_invariant tr_dec);
+      // Should succeed since we are in the Some case
+      assert(Msg2? msg2);
+      let Msg2 msg2 = msg2 in
+      let bob = msg2.bob in
+      let n_a = msg2.n_a in
+      let n_b = msg2.n_b in
+      assert(is_knowable_by (nonce_label alice bob) tr_dec n_b);
+      let (Some(sid, current_state_alice), tr_lookup) = lookup_state #state_t alice
+        (fun current_state_alice -> 
+              SentMsg1? current_state_alice
+          && (SentMsg1?.sentmsg1 current_state_alice).n_a = n_a
+          && (SentMsg1?.sentmsg1 current_state_alice).bob = bob
+        ) tr_rec in
+      assert(trace_invariant tr_lookup);
+      assert(SentMsg1? current_state_alice);
+      let msg3 = Msg3 {n_b} in
+      let (Some(msg3_encrypted), tr_enc) = pke_enc_for alice bob alice_public_keys_sid key_tag msg3 tr_rec in
+      assert(trace_invariant tr_enc);
+      let (msg3_ts, tr_send) = send_msg msg3_encrypted tr_enc in
+      assume(is_publishable tr_enc msg3_encrypted);
+      assert(trace_invariant tr_send);
+      let msg3_state = SentMsg3 {bob; n_a; n_b} in
+      let (_, tr_st) = set_state alice sid msg3_state tr_send in
+      assert(is_knowable_by (nonce_label alice bob) tr n_b);
+      assert(trace_invariant tr_st);
+      ()
+    )
+  )
 
   val receive_msg3:
     alice:principal -> bob:principal -> bob_public_keys_sid:state_id -> bob_private_keys_sid:state_id -> msg3_ts:timestamp -> tr:trace ->
@@ -71,4 +123,4 @@ val receive_msg1_and_send_msg2:
       trace_invariant tr_out
     ))
 
-  let receive_msg3 alice bob bob_public_keys_sid bob_private_keys_sid msg3_ts tr = (admit())
+  let receive_msg3 alice bob bob_public_keys_sid bob_private_keys_sid msg3_ts tr = ()
